\documentclass[11pt]{article}
%\def\hidesolutions{}
\input{header}
\begin{document}
\exsheet{11}{28}{November} % parameters are the number of the session and the day

\begin{exercise}
    The Fourier transform of 
    \begin{align*}
        f(x) = e^{-5x^2}
    \end{align*}
    is the function 
    \begin{align*}
        f(x) = \frac{1}{\sqrt{10}} e^{-\frac{\alpha^2}{20}}.
    \end{align*}
    Find the Fourier transforms of 
    \begin{align*}
     f', \quad f'', \quad f''', \quad f'''', \quad g(x) = f(2x), \quad h(x) = f(x-3).
    \end{align*}
\end{exercise}
\begin{solution}  
To evaluate the Fourier transform of the derivative of a function we will use the following identity from the lecture:
\[
    \mathfrak{F}\left(f^{(n)}\right)(\alpha)=(i \alpha)^n \mathfrak{F}(f)(\alpha)
\]
We then find 
\begin{itemize}
\item $\mathfrak{F}\left(f' \right)(\alpha) = i \alpha \mathfrak{F}(f)(\alpha) = \frac{i \alpha}{\sqrt{10}} e^{-\frac{\alpha^2}{20}}$
\item $\mathfrak{F}\left(f'' \right)(\alpha) = -\alpha^2 \mathfrak{F}(f)(\alpha) = -\frac{ \alpha^2}{\sqrt{10}} e^{-\frac{\alpha^2}{20}}$
\item $\mathfrak{F}\left(f' \right)(\alpha) = -i \alpha^3 \mathfrak{F}(f)(\alpha) = \frac{-i \alpha^3}{\sqrt{10}} e^{-\frac{\alpha^2}{20}}$
\item $\mathfrak{F}\left(f' \right)(\alpha) = \alpha^4 \mathfrak{F}(f)(\alpha) = \frac{ \alpha^4}{\sqrt{10}} e^{-\frac{\alpha^2}{20}}$
\end{itemize}
For the Fourier transform of $g(x)$ we use the following identity from the lecture: 
$g(x)=e^{-i b x} f(a x)$ has the Fourier transform
$\hat{g}(\alpha)=\frac{1}{|a|} \hat{f}\left(\frac{\alpha+b}{a}\right)$,
consequently:
\begin{align*}
    \mathfrak{F}(g(x))(\alpha) & =\mathfrak{F}(f(2 x))(\alpha) \\ & =\frac{1}{2} \mathfrak{F}(f(x))\left(\frac{\alpha}{2}\right) \\ & =\frac{1}{2 \sqrt{10}} e^{-\frac{\left(\frac{\alpha}{2}\right)^2}{20}} \\ & =\frac{1}{2 \sqrt{10}} e^{-\frac{\alpha^2}{80}}
\end{align*}
For the Fourier transform of $h(x)$ we calculate 
\begin{align*}
    \mathfrak{F}(h(x))(x) & =\mathfrak{F}(f(x-3))(\alpha) \\ & =\mathfrak{F}\left(\frac{1}{\sqrt{10}} e^{-5 x^2+30 x-45}\right)(x) \\ & =\mathfrak{F}\left(e^{-45} e^{30 x} f(x)\right)(\alpha) \\ & =e^{-45} \mathfrak{F}\left(e^{-i(30 i) x} f(x)\right)(\alpha) \\ & =e^{-45} \mathfrak{F}(f(x))(\alpha+30 i) \\ & =\frac{e^{-45}}{\sqrt{10}} e^{-\frac{(\alpha+30 i)^2}{20}}
\end{align*}
\end{solution}

\begin{exercise}
    Find $f : \mathbb R \to \mathbb R$ such that 
    \begin{align*}
        \hat f(\alpha) = \frac{3}{1+\alpha^{2}} + \frac{-1}{1+4\alpha^{2}} + \frac{ \sin( 4 \alpha + 3 ) }{ 4 \alpha + 3 }
    \end{align*}
\end{exercise}
\begin{solution}   Because of the linearity property we can treat the inverse of each term in seperately. Therefore 
 \begin{itemize}
\item $\begin{aligned} \mathfrak{F}^{-1}\left(\frac{\sin (4 \alpha+3)}{4 a r+3}\right)(x) & =\frac{\frac{1}{4}}{\frac{1}{4}} \mathfrak{F}^{-1}\left(\frac{\sin \left(\frac{\alpha+3 / 4}{\frac{1}{4}}\right)}{\frac{\alpha+\frac{3}{4}}{\frac{1}{4}}}\right)(x) \\ & =\frac{1}{4} e^{-i \frac{3}{4} x} \sqrt{\frac{\pi}{2}} \mathfrak{F}^{-1}\left(\sqrt{\frac{2}{\pi}} \frac{\sin (\alpha)}{\alpha}\right)\left(\frac{x}{4}\right) \\ & = \begin{cases}\frac{1}{4} \sqrt{\frac{\pi}{2}} e^{-i \frac{3}{4} x} & \text { if }-4 \leq x \leq 4 \\ 0 & \text { else }\end{cases} \end{aligned}$
\item $\begin{aligned} \mathfrak{F}^{-1}\left(\frac{3}{1+\alpha^2}\right)(x) & =3 \sqrt{\frac{\pi}{2}} \mathfrak{F}^{-1}\left(\sqrt{\frac{2}{\pi}} \frac{1}{1+a^2}\right)(x) \\ & =3 \sqrt{\frac{\pi}{2}} e^{-|x|}\end{aligned}$
\item $\begin{aligned} \mathfrak{F}^{-1}\left(\frac{-1}{1+4 \alpha^2}\right)(x) & =-\sqrt{\frac{\pi}{2}} \mathfrak{F}^{-1}\left(\sqrt{\frac{2}{\pi}} \frac{1}{1+(2 \alpha)^2}\right)(x) \\ & =-\sqrt{\frac{\pi}{2}} \frac{\frac{1}{2}}{\frac{1}{2}} \mathfrak{F}^{-1}\left(\sqrt{\frac{2}{\pi}} \frac{1}{1+\left(\frac{\alpha}{\frac{1}{2}}\right)^2}\right)(x \mid \\ & =-\sqrt{\frac{\pi}{2}} \frac{1}{2} \mathfrak{F}^{-1}\left(\sqrt{\frac{2}{\pi}} \frac{1}{1+\alpha^2}\right)\left(\frac{x}{2}\right) \\ & =-\frac{1}{2} \sqrt{\frac{\pi}{2}} e^{-\left|\frac{x}{2}\right|}\end{aligned}$
\end{itemize}

All together this gives

$$
f(x) = \begin{cases}-\frac{1}{2} \sqrt{\frac{\pi}{2}} e^{-\left|\frac{x}{2}\right|}+3 \sqrt{\frac{\pi}{2}} e^{-|x|}+\frac{1}{4} \sqrt{\frac{\pi}{2}} e^{-i \frac{3}{4} x} & -4 \leq x \leq 4 \\ -\frac{1}{2} \sqrt{\frac{\pi}{2}} e^{-\left|\frac{x}{2}\right|}+3 \sqrt{\frac{\pi}{2}} e^{-|x|} & \text { else }\end{cases}
$$
\end{solution}

\begin{exercise}
    Find the Fourier transform of 
    \begin{align*}
        f(x) = \left\{\begin{array}{ll}
                \sin(x) & \text{ if } 0 \leq x \leq 2 \pi 
                \\
                0 & \text{ otherwise }
               \end{array}
               \right.
    \end{align*}
\end{exercise}
\begin{solution} 
$$\begin{aligned} \mathcal{F}(f(x))(\alpha) & =\frac{1}{\sqrt{2 \pi}} \int_0^{2 \pi} \sin x e^{-i \alpha x} d x \\ & =\frac{1}{\sqrt{2 \pi}}\left[\sin x \frac{e^{-i \alpha x}}{-i \alpha}\right]_0^{2 \pi}+\frac{1}{\sqrt{2 \pi}} \int_0^{2 \pi} \frac{\cos x}{i \alpha} e^{-\alpha i x} d x \\ & =\frac{1}{\sqrt{2 \pi}}\left[\frac{\cos x}{a^2} e^{-i \alpha x}\right]_0^{2 \pi}+\frac{1}{\sqrt{2 \pi}} \int_0^{2 \pi} \frac{\sin x}{\alpha^2} e^{-i \alpha x} d x \\ & =\frac{1}{\sqrt{2 \pi} \alpha^2}\left(e^{-2 \pi i \alpha}-1\right)+\frac{1}{\alpha^2} \frac{1}{\sqrt{2 \pi}} \int_0^{2 \pi} \sin x e^{-i \alpha x} d x\end{aligned}$$
$$
\begin{aligned} \Rightarrow \frac{1}{\sqrt{2 \pi}} \int_0^{2 \pi} \sin x e^{-i \alpha x} d x & =\left(\frac{1}{1-\frac{1}{\alpha^2}}\right) \frac{\left(e^{-2 \pi i \alpha}-1\right)}{\sqrt{2 \pi} \alpha^2} \\ & =\frac{\alpha^2}{\alpha^2-1} \frac{\left(e^{-2 \pi i \alpha}-1\right)}{\alpha^2 \sqrt{2 \pi}} \\ & =\frac{\left(e^{-2 \pi i \alpha}-1\right)}{\sqrt{2 \pi}\left(\alpha^2-1\right)}\end{aligned}
$$
\end{solution}

\begin{exercise}
    Find the Laplace transform $F(z)$ of 
    \begin{align*}
        f : \bbR_{0}^{+} \to \bbR, \quad t \mapsto t^{2}.
    \end{align*}
\end{exercise}
\begin{solution}     
We compute 
\begin{align*}
    F(z)&=\int_0^{\infty} t^2 e^{-z t} d t=\left[-\frac{t^2}{z} e^{-z t}\right]_0^{\infty}+\int_0^{\infty} \frac{2 t}{z} e^{-z t} d t \\ &=\left[\frac{2 t}{-z^2} e^{-z t}\right]_0^{\infty}+\int_0^{\infty} \frac{2}{z^2} e^{-z t} d t \\ &=\left[-\frac{2}{z^3} e^{-z t}\right]_0^{\infty} \\ &=0+\frac{2}{z^3} \\ &=\frac{2}{z^3}
    .
\end{align*}
Hence 
\begin{align*}
    F(z)=\frac{2}{z^3} \quad \text { for } \mathrm{R}(z)>0.
\end{align*}
\end{solution}

\begin{exercise}[Extra]
    We have introduced the Fourier transform 
    \begin{align*}
        \frakF(f)(\alpha) := \frac{1}{\sqrt{2\pi}}\int_{-\infty}^{\infty} f(x) e^{-i \alpha x} dx
    \end{align*}
    Different authors define the Fourier transform alternatively by:
    \begin{align*}
        \frakF_2(f)(\xi) 
        := \int_{-\infty}^{\infty} f(x) e^{-i \omega x} dx
        ,
        \quad 
        \frakF_3(f)(\omega) 
        := \int_{-\infty}^{\infty} f(x) e^{-i 2\pi \xi x} dx
        .
    \end{align*}
    Express $\frakF_{2}(f)$ and $\frakF_{3}(f)$ in terms of $\frakF(f)$.
\end{exercise}
\begin{solution}    
    Obviously, 
    \begin{align*}
        \frakF_{2}(f)(\omega) = \frac{1}{\sqrt{2\pi}} \frakF(f)(\omega).
    \end{align*}
    For the other transformation:
    \begin{align*}
        \frakF_3(f)(\omega) 
        &
        = 
        \int_{-\infty}^{\infty} f(x) e^{-i 2\pi \xi x} dx
        = 
        \sqrt{2\pi} 
        \cdot 
        \frac{1}{\sqrt{2\pi}}
        \int_{-\infty}^{\infty} f(x) e^{-i 2\pi \xi x} dx
        = 
        \sqrt{2\pi} 
        \cdot 
        \frakF(f)( 2\pi \xi )
        .
    \end{align*}
\end{solution}

\begin{exercise}
    Compute the Fourier transform of the signal 
    \[
        f(t) = \left\{\begin{array}{ll} e^{t} & \text{ if } -1 \leq t \leq 1 \\ 0 & \text{ otherwise. } \end{array}\right.,
    \]
    and find the Fourier transform of the first to fifth derivative of $f$. 
\end{exercise}
\begin{solution}     
\end{solution}

\begin{exercise}
    Compute the Laplace transform of 
    \[
        f(t) = cos( a t ),
    \]
    where $a > 0$ is a positive number. 
\end{exercise}
\begin{solution}     
    There are different possible approaches. We use the expression of the complex exponential in terms of the cosine and sine function, and we write $z = a + ib$. Then:
\end{solution}

\end{document}
